@prefix dcterms: <http://purl.org/dc/terms/> .
@prefix foaf: <http://xmlns.com/foaf/0.1/> .
@prefix owl: <http://www.w3.org/2002/07/owl#> .
@prefix rdf: <http://www.w3.org/1999/02/22-rdf-syntax-ns#> .
@prefix rdfs: <http://www.w3.org/2000/01/rdf-schema#> .
@prefix skos: <http://www.w3.org/2004/02/skos/core#> .
@prefix xapi: <https://w3id.org/xapi/ontology#> .
@prefix xml: <http://www.w3.org/XML/1998/namespace> .
@prefix xsd: <http://www.w3.org/2001/XMLSchema#> .

xapi: a owl:Ontology ;
    rdfs:label "xAPI Ontology"@en ;
    dcterms:created "2015-11-19"^^xsd:date ;
    dcterms:modified "2017-04-13"^^xsd:date ;
    rdfs:comment "This ontology contains the classes and properties that are used when for semantically expressing the structure and relationships of xAPI data."@en .

xapi:AllDisjointClasses a owl:AllDisjointClasses ;
    owl:members ( xapi:Actor xapi:Verb xapi:Object xapi:Context xapi:Result) .

#################################################################
### Statement Classes 
#################################################################
      
xapi:Statement a owl:Class ;
	rdfs:label "Statement"@en ;
	rdfs:comment "The Class used to represent a Statement object in xAPI."@en .


#################################################################
### Statement Properties
#################################################################

xapi:stored a owl:DatatypeProperty ;
	rdfs:label "stored"@en ;
	rdfs:comment "The time at which a Statement is stored by the LRS. This can be any time between when the LRS receives the Statement and when it is written to storage. Formatted in milliseconds according to ISO 8601's normal format."@en ;
	rdfs:domain xapi:Statement ;
	rdfs:range xsd:dateTime .	
	
xapi:timeStamp a owl:DatatypeProperty ;
	rdfs:label "timeStamp"@en ;
	rdfs:comment "Timestamps represent a specific time and are formatted in milliseconds according to ISO 8601's normal format."@en ;
	rdfs:domain xapi:Statement ;
	rdfs:range xsd:dateTime .
	
xapi:version a owl:AnnotationProperty ;
	rdfs:label "version"@en ;
	rdfs:comment "The Statementâ€™s associated xAPI version, formatted according to Semantic Versioning 1.0.0." ;
	rdfs:domain xapi:Statement ;
	rdfs:range xsd:string .	
	
#################################################################	
### Actor Classes 
#################################################################    

xapi:Actor a owl:Class ;
	rdfs:label "Actor"@en ;
	rdfs:comment "The Class used for the Actor object in xAPI."@en ;
	rdfs:subClassOf xapi:Statement .   
	
xapi:Agent a owl:Class ;
	rdfs:label "Agent"@en ;
	rdfs:comment "The Class used for the Agent object in xAPI."@en ;
	rdfs:subClassOf xapi:Actor .

xapi:Account a owl:Class ;
	rdfs:label "Account"@en ;
	rdfs:comment "The Class used for the Account object in xAPI."@en ; 
	rdfs:subClassOf xapi:Actor .
	
xapi:AnonymousGroup a owl:Class ;
	rdfs:label "AnonymousGroup"@en ;
	rdfs:comment "The Class used for an Anonymous Group object in xAPI."@en ;
	rdfs:subClassOf xapi:Actor .  
	
xapi:IdentifiedGroup a owl:Class ;
	rdfs:label "Group"@en ;
	rdfs:comment "The Class used for an Identified Group object in xAPI."@en ; 
	rdfs:subClassOf xapi:Actor .  	

#################################################################
### Actor Properties
#################################################################

xapi:mbox a owl:DatatypeProperty ;
	rdfs:label "mbox"@en ;
	rdfs:comment "The required format is mailto:user@emailaddress. Only email addresses that have only ever been and will ever be assigned to this Agent, but no others, SHOULD be used for this property and mbox_sha1sum." ;
	rdfs:domain xapi:Actor ;
	rdfs:subPropertyOf foaf:mbox .

xapi:mbox_sha1sum a owl:DatatypeProperty ;
	rdfs:label "mbox_sha1sum"@en ;
	rdfs:comment "The hex-encoded SHA1 hash of a mailto IRI (i.e. the value of an mbox property). An LRS MAY include Agents with a matching hash when a request is based on an mbox." ;
	rdfs:domain xapi:Actor ;
	rdfs:subPropertyOf foaf:mbox_sha1sum .

xapi:openid a owl:DatatypeProperty ;
	rdfs:label "openid"@en ;
	rdfs:comment "An openID that uniquely identifies the Agent." ;
	rdfs:domain xapi:Actor ;
	rdfs:range xsd:anyURI .
	
xapi:homePage a owl:DatatypeProperty ;
	rdfs:label "homePage"@en ;
	rdfs:comment "The canonical home page for the system the account is on. This is based on FOAF's accountServiceHomePage." ;
	rdfs:domain xapi:Account ;
	rdfs:range xsd:anyURI ;
	rdfs:subPropertyOf foaf:accountServiceHomepage .


#################################################################	
### Verb Classes 
#################################################################

xapi:Verb a owl:Class ;
    rdfs:label "Verb"@en ;
    rdfs:comment "The Class used for a Verb object in xAPI."@en ;
    rdfs:subClassOf skos:Concept ;
    rdfs:subClassOf xapi:Statement .
    
#################################################################    
### Verb Properties    
################################################################# 


# All Classes
xapi:ActivityType a owl:Class ;
    rdfs:label "ActivityType"@en ;
    rdfs:comment "The Class for a Activity Type in an xAPI vocabulary or profile."@en ;
    rdfs:subClassOf skos:Concept .

xapi:Extension a owl:Class ;
    rdfs:label "Extension"@en ;
    rdfs:comment "The Class for an Extension in an xAPI vocabulary or profile."@en ;
    rdfs:subClassOf skos:Concept .

xapi:Verb a owl:Class ;
    rdfs:label "Verb"@en ;
    rdfs:comment "The Class for a Verb in an xAPI vocabulary or profile."@en ;
    rdfs:subClassOf skos:Concept .

# All Properties
xapi:closelyRelatedNaturalLanguageTerm a owl:ObjectProperty ;
    rdfs:label "closelyRelatedNaturalLanguageTerm"@en ;
    rdfs:comment "A property used to connect the xAPI term to a specific sense, or meaning, in natural language that is very closely related. The sense will be identified with Wordnet, a carefully constructed ontology that aids in word sense disambiguation, which has been used with many different languages."@en ;
    rdfs:domain skos:Concept ;
    rdfs:range <http://wordnet-rdf.princeton.edu/ontology#Synset> ;
    rdfs:subPropertyOf skos:relatedMatch .    

xapi:referencedBy a owl:ObjectProperty ;
    rdfs:label "referencedBy"@en ;
    rdfs:comment "A property used to connects an xapi:Verb not directly maintained by the vocabulary author to a vocabulary that is reusing and referencing the term."@en ;
    rdfs:range skos:ConceptScheme ;
    rdfs:subPropertyOf skos:inScheme .

xapi:thirdPartyLabel a owl:AnnotationProperty ;
    rdfs:label "thirdPartyLabel"@en ;
    rdfs:comment "A property used by people who did not create the original verb, but would like to offer an alternative label for it."@en ;
    rdfs:subPropertyOf skos:altLabel .
    
#################################################################            
### Object/Activity Classes
#################################################################

xapi:Object a owl:Class ;
	rdfs:label "Object"@en ;
	rdfs:comment "The Class used for the Object in xAPI."@en ;
	rdfs:subClassOf xapi:Statement .

xapi:Activity a owl:Class ;
	rdfs:label "Activity"@en ;
	rdfs:comment "The Class used for the Activity Object in xAPI."@en ;
	rdfs:subClassOf xapi:Object . 
	
xapi:ActivityDefinition a owl:Class ;
	rdfs:label "Activity"@en ;
	rdfs:comment "The Class used for the ActivityDefinition object in xAPI."@en ;
	rdfs:subClassOf xapi:Activity . 	 

<<<<<<< Updated upstream

=======
xapi:ActivityType a owl:Class ;
    rdfs:label "ActivityType"@en ;
    rdfs:comment "The Class for an Activity Type in an xAPI vocabulary or profile."@en ;
    rdfs:subClassOf skos:Concept ;
    rdfs:subClassOf xapi:ActivityDefinition .
      
	
#################################################################
### Object/Activity Properties
#################################################################	

xapi:StatementRef a owl:ObjectProperty ;
	rdfs:label "StatementRef"@en ;
	rdfs:comment "The Class used for a Statement Reference object in xAPI."@en .
	
xapi:SubStatement a owl:ObjectProperty ;
	rdfs:label "SubStatement"@en ;
	rdfs:comment "The Class used for a Sub Statement object in xAPI."@en . 		

#################################################################		
### Result Classes
#################################################################

xapi:Result a owl:Class ;
	rdfs:label "Result"@en ;
	rdfs:comment "The Class used for a Result object in xAPI."@en ;
	rdfs:subClassOf xapi:Statement .

xapi:Score a owl:Class ;
	rdfs:label "Result"@en ;
	rdfs:comment "The Class used for a Score object in xAPI."@en ;
	rdfs:subClassof xapi:Result .

#################################################################	
### Result Properties	
#################################################################

xapi:completion a owl:DatatypeProperty ;
	rdfs:label "completion"@en ;
	rdfs:comment "A property used to provide the completion status (true or false) of a Result object in xAPI."@en ;
	rdfs:domain xapi:Result ;
	rdfs:range xsd:boolean .

xapi:duration a owl:DatatypeProperty ;
    rdfs:label "duration"@en ;
    rdfs:comment "Period of time over which the Statement occurred. Formatted according to ISO 8601 with a precision of 0.01 seconds"@en ;
    rdfs:domain xapi:Result ;
    rdfs:range xsd:duration .

xapi:response a owl:DatatypeProperty ;
	rdfs:label "response"@en ;
	rdfs:comment "A property used to provide a textual response in the Result object."@en ;
	rdfs:domain xapi:Result ;
	rdfs:range xsd:string .    

xapi:success a owl:DatatypeProperty ;
	rdfs:label "success"@en ;
	rdfs:comment "A property used to provide the success status (true or false) of a Result object in xAPI."@en ;
	rdfs:domain xapi:Result ;
	rdfs:range xsd:boolean .	

#################################################################	
### Context Classes 
#################################################################

xapi:Context a owl:Class ;
	rdfs:label "Context"@en ;
	rdfs:comment "The Class used for an Context object in xAPI."@en ;
	rdfs:subClassOf xapi:Statement . 

xapi:ContextActivities a owl:Class ;
	rdfs:label "ContextActivities"@en ;
	rdfs:comment "The Class used for a ContextActivities object in xAPI."@en ;
	rdfs:subClassOf xapi:Context . 
		

#################################################################
### Context Properties	
#################################################################

xapi:registration a owl:DatatypeProperty ;
	rdfs:label "registration"@en ;
	rdfs:comment "A property used to provide the registration identifier of a Context object in xAPI."@en ;
	rdfs:domain xapi:Context .

#################################################################		
### Authority Classes 
#################################################################

xapi:Authority a owl:ObjectProperty ;
	rdfs:label "Authority"@en ;
	rdfs:comment "The Class used for the Authority object in xAPI. The Authority is the Agent or Group who is asserting this Statement is true. Verified by the LRS based on authentication. Set by LRS if not provided or if a strong trust relationship between the Learning Record Provider and LRS has not been established."@en .
	
#################################################################
### Authority Properties
#################################################################

#################################################################
### Attachment Classes 
#################################################################

#################################################################
### Attachment Properties
#################################################################
    
#################################################################
# Unions
#################################################################
xapi:NamePropertyUnion a owl:Class ;
	rdfs:label "NamePropertyUnion"@en ;
	rdfs:comment "The Class used to create a multiple domain axiom for the name property so it can be used with multiple Classes."@en ;
	owl:unionOf (xapi:Agent xapi:Account xapi:AnonymousGroup xapi:IdentifiedGroup xapi:ActivityDefinition xapi:StatementRef) .    

xapi:name a owl:DatatypeProperty ;
	rdfs:label "name"@en ;
	rdfs:comment "A property used to provide the name of an object in xAPI."@en ;
	rdfs:domain xapi:NamePropertyUnion ;
	rdfs:range xsd:string .
	
xapi:DescriptionPropertyUnion a owl:Class ;
	rdfs:label "DescriptionPropertyUnion"@en ;
	rdfs:comment "The Class used to create a multiple domain axiom for the description property so it can be used with multiple Classes."@en ;
	owl:unionOf (xapi:ActivityDefinition xapi:Attachment) .    

xapi:description a owl:DatatypeProperty ;
	rdfs:label "description"@en ;
	rdfs:comment "A property used to provide the name of an object in xAPI."@en ;
	rdfs:domain xapi:DescriptionPropertyUnion ;
	rdfs:range xsd:string .

xapi:ExtensionsUnion a owl:Class ;
	rdfs:label "ExtensionsUnion"@en ;
	rdfs:comment "The Class used to create a multiple domain axiom for the extensions property so it can be used with multiple Classes."@en ;
	owl:unionOf (xapi:Activity xapi:Result xapi:Context) .    

xapi:extensions a owl:ObjectProperty ;
	rdfs:label "extensions"@en ;
	rdfs:comment "A property used to define the extensions object in xAPI."@en ;
	rdfs:domain xapi:ExtensionsUnion .

xapi:MemberUnion a owl:Class ;
	rdfs:label "MemberUnion"@en ;
	rdfs:comment "The Class used to create a multiple domain axiom for the member property so it can be used with multiple Classes."@en ;
	owl:unionOf (xapi:AnonymousGroup xapi:IdentifiedGroup) .    

xapi:member a owl:DatatypeProperty ;
	rdfs:label "member"@en ;
	rdfs:comment "A property used to provide the members of a group object in xAPI."@en ;
	rdfs:domain xapi:MemberUnion .
>>>>>>> Stashed changes



